src/coqutil/Map/Empty_set_keyed_map.v
@@ -7,7 +7,7 @@ Instance map(V: Type): map.map Empty_set V := {|
   map.empty := tt;
   map.put m := Empty_set_rect _;
   map.remove m := Empty_set_rect _;
-  map.putmany m1 m2 := tt;
+  map.fold R f r0 m := r0;
 |}.
 
 Local Set Default Goal Selector "all".
@@ -20,5 +20,5 @@ Proof.
          | m: map.rep |- _ => destruct m
          | x: Empty_set |- _ => destruct x
          end.
-  reflexivity.
+  reflexivity || assumption.
 Qed.
